docs/verification/phonetic/rewrite_rules.v
@@ -13,7 +13,8 @@
     Reference: https://zompist.com/spell.html
 *)
 
-Require Import String List Arith QArith Ascii Bool.
+Require Import String List Arith QArith ZArith Ascii Bool.
+Require Import Coq.Lists.ListDec.
 Import ListNotations.
 
 (** * Core Definitions *)
@@ -40,6 +41,34 @@ Inductive Context : Set :=
   | BeforeConsonant : list ascii -> Context    (** Before specific consonants: _C *)
   | AfterVowel : list ascii -> Context         (** After specific vowels: V_ *)
   | Anywhere : Context.                        (** No positional restriction *)
+
+(** Decidable equality for ascii *)
+Definition Ascii_eq_dec (c1 c2 : ascii) : {c1 = c2} + {c1 <> c2}.
+Proof.
+  destruct (Ascii.eqb c1 c2) eqn:E.
+  - left. apply Ascii.eqb_eq. exact E.
+  - right. intro H. subst. rewrite Ascii.eqb_refl in E. discriminate.
+Defined.
+
+(** Decidable equality for ascii lists *)
+Definition ascii_list_eq_dec : forall (l1 l2 : list ascii), {l1 = l2} + {l1 <> l2}.
+Proof.
+  apply list_eq_dec. exact Ascii_eq_dec.
+Defined.
+
+(** Context has decidable equality *)
+Definition Context_eq_dec (c1 c2 : Context) : {c1 = c2} + {c1 <> c2}.
+Proof.
+  destruct c1, c2; try (left; reflexivity); try (right; discriminate).
+  - (* BeforeVowel vs BeforeVowel *)
+    destruct (ascii_list_eq_dec l l0); [left | right]; congruence.
+  - (* AfterConsonant vs AfterConsonant *)
+    destruct (ascii_list_eq_dec l l0); [left | right]; congruence.
+  - (* BeforeConsonant vs BeforeConsonant *)
+    destruct (ascii_list_eq_dec l l0); [left | right]; congruence.
+  - (* AfterVowel vs AfterVowel *)
+    destruct (ascii_list_eq_dec l l0); [left | right]; congruence.
+Defined.
 
 (** ** Rewrite Rule *)
 
@@ -114,6 +143,84 @@ Proof.
   (* Digraph case *)
   f_equal; apply Ascii.eqb_sym.
 Qed.
+
+(** Phone_eqb reflects equality *)
+Lemma Phone_eqb_spec : forall p1 p2, reflect (p1 = p2) (Phone_eqb p1 p2).
+Proof.
+  intros p1 p2.
+  destruct p1, p2; simpl; try (constructor; discriminate).
+  - (* Vowel vs Vowel *)
+    destruct (Ascii.eqb_spec a a0); constructor; congruence.
+  - (* Consonant vs Consonant *)
+    destruct (Ascii.eqb_spec a a0); constructor; congruence.
+  - (* Digraph vs Digraph *)
+    destruct (Ascii.eqb_spec a a1), (Ascii.eqb_spec a0 a2);
+    simpl; constructor;
+    try (subst; reflexivity);
+    intro H; injection H; intros; subst; contradiction.
+  - (* Silent vs Silent *)
+    constructor. reflexivity.
+Qed.
+
+(** Phone has decidable equality *)
+Definition Phone_eq_dec (p1 p2 : Phone) : {p1 = p2} + {p1 <> p2}.
+Proof.
+  destruct (Phone_eqb p1 p2) eqn:E.
+  - left. destruct (Phone_eqb_spec p1 p2); [assumption | discriminate].
+  - right. destruct (Phone_eqb_spec p1 p2); [discriminate | assumption].
+Defined.
+
+(** ** Complete Decidable Equality for RewriteRule *)
+
+(** Decidable equality for Q (Leibniz equality, not Qeq) *)
+Definition Q_leibniz_eq_dec (q1 q2 : Q) : {q1 = q2} + {q1 <> q2}.
+Proof.
+  destruct q1 as [n1 d1].
+  destruct q2 as [n2 d2].
+  destruct (Z.eq_dec n1 n2) as [H_n_eq | H_n_neq];
+  destruct (Pos.eq_dec d1 d2) as [H_d_eq | H_d_neq].
+  - left. subst. reflexivity.
+  - right. intro H. injection H. intros. contradiction.
+  - right. intro H. injection H. intros. contradiction.
+  - right. intro H. injection H. intros. contradiction.
+Defined.
+
+(** Decidable equality for string *)
+Definition string_eq_dec (s1 s2 : string) : {s1 = s2} + {s1 <> s2}.
+Proof.
+  generalize dependent s2.
+  induction s1 as [| c1 s1' IH]; intros s2.
+  - destruct s2.
+    + left. reflexivity.
+    + right. discriminate.
+  - destruct s2 as [| c2 s2'].
+    + right. discriminate.
+    + destruct (Ascii_eq_dec c1 c2) as [H_c_eq | H_c_neq].
+      * destruct (IH s2') as [H_s_eq | H_s_neq].
+        ** left. subst. reflexivity.
+        ** right. intro H. injection H. intros. contradiction.
+      * right. intro H. injection H. intros. contradiction.
+Defined.
+
+(** Decidable equality for PhoneticString (list Phone) *)
+Definition PhoneticString_eq_dec (s1 s2 : PhoneticString) : {s1 = s2} + {s1 <> s2}.
+Proof.
+  apply list_eq_dec. exact Phone_eq_dec.
+Defined.
+
+(** RewriteRule has decidable equality - derived from field types, NO AXIOM *)
+Definition RewriteRule_eq_dec (r1 r2 : RewriteRule) : {r1 = r2} + {r1 <> r2}.
+Proof.
+  destruct r1 as [id1 name1 pat1 repl1 ctx1 wt1].
+  destruct r2 as [id2 name2 pat2 repl2 ctx2 wt2].
+  destruct (Nat.eq_dec id1 id2); [| right; congruence].
+  destruct (string_eq_dec name1 name2); [| right; congruence].
+  destruct (PhoneticString_eq_dec pat1 pat2); [| right; congruence].
+  destruct (PhoneticString_eq_dec repl1 repl2); [| right; congruence].
+  destruct (Context_eq_dec ctx1 ctx2); [| right; congruence].
+  destruct (Q_leibniz_eq_dec wt1 wt2); [| right; congruence].
+  left. subst. reflexivity.
+Defined.
 
 (** Check if an option is Some *)
 Definition is_Some {A : Type} (o : option A) : bool :=
